refactor(Neighborhood): Canonicity (#589)

Foundation/Modal/Neighborhood/Completeness.lean
@@ -18,7 +18,18 @@ abbrev Proofset (𝓢 : S) := Set (MaximalConsistentSet 𝓢)
 
 def proofset (𝓢 : S) (φ : Formula α) : Proofset 𝓢 := { Γ : MaximalConsistentSet 𝓢 | φ ∈ Γ }
 
-def Nonproofset (𝓢 : S) := { P : Proofset 𝓢 // ∀ φ, P ≠ proofset 𝓢 φ }
+def Proofset.IsNonproofset {𝓢 : S} (P : Proofset 𝓢) := ∀ φ, P ≠ proofset 𝓢 φ
+
+omit [DecidableEq α] [Entailment.Cl 𝓢] in
+lemma iff_not_isNonProofset_exists : ¬P.IsNonproofset ↔ ∃ φ, P = proofset 𝓢 φ := by
+  dsimp [Proofset.IsNonproofset];
+  push_neg;
+  tauto;
+
+omit [DecidableEq α] [Entailment.Cl 𝓢] in
+@[simp]
+lemma not_isNonproofset_proofset : ¬(proofset 𝓢 φ).IsNonproofset := by simp [Proofset.IsNonproofset];
+
 
 namespace proofset
 
@@ -203,7 +214,7 @@ lemma completeness {C : FrameClass} (hC : 𝓒.toModel.toFrame ∈ C) : LO.Compl
 end Canonicity
 
 
-def minimalCanonicity (𝓢 : S) [Entailment.E 𝓢] : Canonicity 𝓢 where
+def basicCanonicity (𝓢 : S) [Entailment.E 𝓢] : Canonicity 𝓢 where
   𝒩 Γ X := ∃ φ, □φ ∈ Γ ∧ X = proofset 𝓢 φ
   def_𝒩 := by
     intro X φ;
@@ -216,9 +227,10 @@ def minimalCanonicity (𝓢 : S) [Entailment.E 𝓢] : Canonicity 𝓢 where
   V a := proofset 𝓢 (.atom a);
   def_V := by simp;
 
+namespace basicCanonicity
 
-lemma minimalCanonicity.iff_mem_box_exists_fml {X} {Γ : (minimalCanonicity 𝓢).toModel}
-  : Γ ∈ Frame.box _ X ↔ ∃ φ, X = proofset 𝓢 φ ∧ Frame.box _ X = proofset 𝓢 (□φ) ∧ Γ ∈ proofset 𝓢 (□φ)
+lemma iff_mem_box_exists_fml {X A}
+  : A ∈ (basicCanonicity 𝓢).toModel.box X ↔ ∃ φ, X = proofset 𝓢 φ ∧ A ∈ proofset 𝓢 (□φ)
   := by
     constructor;
     . rintro ⟨φ, _, rfl⟩;
@@ -226,14 +238,78 @@ lemma minimalCanonicity.iff_mem_box_exists_fml {X} {Γ : (minimalCanonicity 𝓢
       simpa;
     . tauto;
 
-lemma minimalCanonicity.iff_mem_dia_forall_fml {X} {Γ : (minimalCanonicity 𝓢).toModel}
-  : Γ ∈ Frame.dia _ X ↔ ∀ φ, Xᶜ ≠ proofset 𝓢 φ ∨ Frame.box _ Xᶜ ≠ proofset 𝓢 (□φ) ∨ Γ ∉ proofset 𝓢 (□φ)
+@[grind]
+lemma not_isNonproofset_of_mem_box {X : Proofset 𝓢} (h : A ∈ (basicCanonicity 𝓢).toModel.box X) : ¬X.IsNonproofset := by
+  obtain ⟨φ, rfl, _⟩ := basicCanonicity.iff_mem_box_exists_fml.mp h;
+  simp;
+
+lemma iff_mem_dia_forall_fml {X} {Γ : (basicCanonicity 𝓢).toModel}
+  : Γ ∈ (basicCanonicity 𝓢).toModel.dia X ↔ ∀ φ, Xᶜ ≠ proofset 𝓢 φ ∨ Γ ∉ proofset 𝓢 (□φ)
   := by
     apply Iff.trans (iff_mem_box_exists_fml.not);
     set_option push_neg.use_distrib true in push_neg;
     rfl;
 
-end Neighborhood
+end basicCanonicity
 
+
+
+/-- `basicCanonicity` with condition for non-proofset -/
+def relativeBasicCanonicity (𝓢 : S) [Entailment.E 𝓢] (P : MaximalConsistentSet 𝓢 → Set (Proofset 𝓢)) : Canonicity 𝓢 where
+  𝒩 A (X : Proofset 𝓢) := (basicCanonicity 𝓢 |>.𝒩 A X) ∨ (X.IsNonproofset ∧ X ∈ P A);
+  def_𝒩 := by
+    intro X φ;
+    constructor;
+    . intro h;
+      left;
+      use φ;
+    . rintro (⟨ψ, hψ₁, hψ₂⟩ | h);
+      . have := proofset.eq_boxed_of_eq hψ₂;
+        grind;
+      . simpa using h.1 φ;
+  V a := proofset 𝓢 (.atom a);
+  def_V := by simp;
+
+namespace relativeBasicCanonicity
+
+variable {P} {X : Proofset 𝓢} {A}
+
+protected lemma iff_mem_box :
+  (A ∈ (relativeBasicCanonicity 𝓢 P).toModel.box X) ↔
+  ((A ∈ (basicCanonicity 𝓢).toModel.box X) ∨ (X.IsNonproofset ∧ X ∈ P A)) := by
+  constructor;
+  . rintro (h | h);
+    . left; exact h;
+    . right; exact h;
+  . rintro (h | ⟨h₁, h₂⟩);
+    . left; exact h;
+    . right;
+      constructor;
+      . assumption;
+      . assumption;
+
+protected lemma iff_mem_dia :
+  (A ∈ (relativeBasicCanonicity 𝓢 P).toModel.dia X) ↔
+  ((A ∉ (basicCanonicity 𝓢).toModel.box Xᶜ) ∧ ((¬Xᶜ.IsNonproofset) ∨ Xᶜ ∉ P A)) := by
+  suffices A ∉ ((relativeBasicCanonicity 𝓢 P).toModel.box Xᶜ) ↔ A ∉ (basicCanonicity 𝓢).toModel.box Xᶜ ∧ ((¬Xᶜ.IsNonproofset) ∨ Xᶜ ∉ P A) by
+    simpa [Frame.dia];
+  rw [relativeBasicCanonicity.iff_mem_box.not, Proofset.IsNonproofset]
+  set_option push_neg.use_distrib true in push_neg;
+  tauto;
+
+end relativeBasicCanonicity
+
+abbrev minimalRelativeMaximalCanonicity (𝓢 : S) [Entailment.E 𝓢] : Canonicity 𝓢 := relativeBasicCanonicity 𝓢 (λ _ _ => False)
+
+lemma minimalRelativeMaximalCanonicity.iff_minimal : A ∈ (minimalRelativeMaximalCanonicity 𝓢).toModel.box X ↔ A ∈ (basicCanonicity 𝓢).toModel.box X := by
+  constructor;
+  . rintro (h | ⟨h, _⟩);
+    . exact h;
+    . contradiction;
+  . intro h; left; exact h;
+
+abbrev maximalRelativeMaximalCanonicity (𝓢 : S) [Entailment.E 𝓢] : Canonicity 𝓢 := relativeBasicCanonicity 𝓢 (λ _ _ => True)
+
+end Neighborhood
 
 end LO.Modal
