Foundation/Modal/Neighborhood/Logic/EMCN4.lean
@@ -30,7 +30,7 @@ instance consistent : Entailment.Consistent Modal.EMCN4 := consistent_of_sound_f
   simp only [Set.mem_setOf_eq];
   constructor;
 
-instance Neighborhood.complete : Complete Modal.EMCN4 FrameClass.EMCN4 := (supplementedMinimalCanonicity Modal.EMCN4).completeness $ by
+instance Neighborhood.complete : Complete Modal.EMCN4 FrameClass.EMCN4 := (supplementedBasicCanonicity Modal.EMCN4).completeness $ by
   apply Set.mem_setOf_eq.mpr;
   constructor;
 
